src/Language/PlutusIR/Transform/Compat.v
@@ -10,185 +10,199 @@ From PlutusCert Require Import
   Analysis.Equality
   .
 
-Generalizable All Variables.
-
 Import NamedTerm.
 
 Section Compatibility.
-    Context
+
+  Context
     (R : Term -> Term -> Type)
     (dec_R : Term -> Term -> bool)
   .
 
-
   Inductive Compat_Binding : Binding -> Binding -> Type :=
-    | C_TermBind     : `{ R t t' -> Compat_Binding (TermBind s v t)
-                                                 (TermBind s v t') }
+    | C_TermBind     : ∀ s v t t',
+        R t t' -> Compat_Binding (TermBind s v t) (TermBind s v t')
 
-    | C_TypeBind     : `{           Compat_Binding (TypeBind d T)
-                                                 (TypeBind d T) }
-    | C_DatatypeBind : `{           Compat_Binding (DatatypeBind d)
-                                                   (DatatypeBind d) }
+    | C_TypeBind     : ∀ d T,
+        Compat_Binding (TypeBind d T) (TypeBind d T)
+
+    | C_DatatypeBind : ∀ d,
+        Compat_Binding (DatatypeBind d) (DatatypeBind d)
     .
+
   Inductive Compat_Bindings : list Binding -> list Binding -> Type :=
-    | Compat_Bindings_Cons : forall {b b' bs bs'}, Compat_Binding b b' -> Compat_Bindings bs bs' -> Compat_Bindings (b :: bs) (b' :: bs')
-    | Compat_Bindings_Nil  : Compat_Bindings nil nil.
+    | Compat_Bindings_Cons : ∀ {b b' bs bs'},
+        Compat_Binding b b' -> Compat_Bindings bs bs' -> Compat_Bindings (b :: bs) (b' :: bs')
+
+    | Compat_Bindings_Nil :
+        Compat_Bindings nil nil.
 
   Inductive Compat : Term -> Term -> Type :=
-    | C_Let      : `{ Compat_Bindings bs bs' -> R t t'    -> Compat (Let r bs t)
-                                                                (Let r bs' t')}
-    | C_Var      : `{                          Compat (Var n)
-                                                    (Var n) }
-    | C_TyAbs    : `{ R t t'                -> Compat (TyAbs n k t)
-                                                    (TyAbs n k t') }
-    | C_LamAbs   : `{ R t t' ->                Compat (LamAbs n T t)
-                                                    (LamAbs n T t') }
-    | C_Apply    : `{ R s s' -> R t t'      -> Compat (Apply s t)
-                                                    (Apply s' t')}
-    | C_Constant : `{                          Compat (Constant v)
-                                                    (Constant v) }
-    | C_Builtin  : `{                          Compat (Builtin f)
-                                                    (Builtin f)}
-    | C_TyInst   : `{ R t t'                -> Compat (TyInst t T)
-                                                    (TyInst t' T)}
-    | C_Error    : `{                          Compat (Error T)
-                                                    (Error T)}
-    | C_IWrap    : `{ R t t'                -> Compat (IWrap T1 T2 t)
-                                                    (IWrap T1 T2 t') }
-    | C_Unwrap   : `{ R t t'                -> Compat (Unwrap t)
-                                                    (Unwrap t')}
+    | C_Let : ∀ bs bs' r t t',
+        Compat_Bindings bs bs' -> R t t' -> Compat (Let r bs t) (Let r bs' t')
+
+    | C_Var : ∀ n,
+        Compat (Var n) (Var n)
+
+    | C_TyAbs : ∀ n k t t',
+        R t t' -> Compat (TyAbs n k t) (TyAbs n k t')
+
+    | C_LamAbs : ∀ n T t t' ,
+        R t t' -> Compat (LamAbs n T t) (LamAbs n T t')
+
+    | C_Apply : ∀ s s' t t' ,
+        R s s' -> R t t' -> Compat (Apply s t) (Apply s' t')
+
+    | C_Constant : ∀ v,
+        Compat (Constant v) (Constant v)
+
+    | C_Builtin : ∀ f,
+        Compat (Builtin f) (Builtin f)
+
+    | C_TyInst : ∀ t t' T,
+        R t t' -> Compat (TyInst t T) (TyInst t' T)
+
+    | C_Error : ∀ T,
+        Compat (Error T) (Error T)
+
+    | C_IWrap : ∀ T1 T2 t t',
+        R t t' -> Compat (IWrap T1 T2 t) (IWrap T1 T2 t')
+
+    | C_Unwrap : ∀ t t',
+        R t t' -> Compat (Unwrap t) (Unwrap t')
   .
-    Definition is_cong_binding  (b b' : Binding) : bool :=
-      match b, b' with
-        | (TermBind s v t), (TermBind s' v' t') => Strictness_eqb s s' && VDecl_eqb v v' && dec_R t t'
-        | (TypeBind v T), (TypeBind v' T') => TVDecl_eqb v v'  && Ty_eqb T T'
-        | (DatatypeBind d), (DatatypeBind d') => DTDecl_eqb d d'
-        | _, _                               => false
-      end
+
+  Definition dec_compat_binding  (b b' : Binding) : bool :=
+    match b, b' with
+      | (TermBind s v t), (TermBind s' v' t') => Strictness_eqb s s' && VDecl_eqb v v' && dec_R t t'
+      | (TypeBind v T), (TypeBind v' T') => TVDecl_eqb v v'  && Ty_eqb T T'
+      | (DatatypeBind d), (DatatypeBind d') => DTDecl_eqb d d'
+      | _, _                               => false
+    end
+  .
+
+
+  Definition dec_compat (t t' : Term) : bool :=
+    match t, t' with
+      | (Let r bs t), (Let r' bs' t')      => Recursivity_eqb r r' && forall2b dec_compat_binding bs bs' && dec_R t t'
+      | (Var n), (Var n')                  => String.eqb n n'
+      | (TyAbs n k t), (TyAbs n' k' t')    => String.eqb n n' && Kind_eqb k k' && dec_R t t'
+      | (LamAbs n T t), (LamAbs n' T' t')  => String.eqb n n'&& Ty_eqb T T' && dec_R t t'
+      | (Apply s t), (Apply s' t')         => dec_R s s' && dec_R t t'
+      | (Constant v), (Constant v')        => some_valueOf_eqb v v'
+      | (Builtin f), (Builtin f')          => func_eqb f f'
+      | (TyInst t T), (TyInst t' T')       => Ty_eqb T T' && dec_R t t'
+      | (Error T), (Error T')              => Ty_eqb T T'
+      | (IWrap T1 T2 t), (IWrap T1' T2' t') => Ty_eqb T1 T1' && Ty_eqb T2 T2' && dec_R t t'
+      | (Unwrap t), (Unwrap t')            => dec_R t t'
+      | _, _                               => false
+    end
     .
 
+  Ltac split_hypos :=
+    match goal with
+    | H : (?x && ?y)%bool = true |- _ => apply andb_true_iff in H; destruct H; split_hypos
+    | _ => idtac
+    end.
 
-    Definition is_cong (t t' : Term) : bool :=
-      match t, t' with
-        | (Let r bs t), (Let r' bs' t')      => Recursivity_eqb r r' && forall2b is_cong_binding bs bs' && dec_R t t'
-        | (Var n), (Var n')                  => String.eqb n n'
-        | (TyAbs n k t), (TyAbs n' k' t')    => String.eqb n n' && Kind_eqb k k' && dec_R t t'
-        | (LamAbs n T t), (LamAbs n' T' t')  => String.eqb n n'&& Ty_eqb T T' && dec_R t t'
-        | (Apply s t), (Apply s' t')         => dec_R s s' && dec_R t t'
-        | (Constant v), (Constant v')        => some_valueOf_eqb v v'
-        | (Builtin f), (Builtin f')          => func_eqb f f'
-        | (TyInst t T), (TyInst t' T')       => Ty_eqb T T' && dec_R t t'
-        | (Error T), (Error T')              => Ty_eqb T T'
-        | (IWrap T1 T2 t), (IWrap T1' T2' t') => Ty_eqb T1 T1' && Ty_eqb T2 T2' && dec_R t t'
-        | (Unwrap t), (Unwrap t')            => dec_R t t'
-        | _, _                               => false
-      end
-      .
-
-    Ltac split_hypos :=
-      match goal with
-      | H : (?x && ?y)%bool = true |- _ => apply andb_true_iff in H; destruct H; split_hypos
-      | _ => idtac
-      end.
-
-    Create HintDb Hints_soundness.
-    Hint Resolve
-      string_eqb_eq
-      Recursivity_eqb_eq
-      Strictness_eqb_eq
-      Kind_eqb_eq
-      Ty_eqb_eq
-      some_valueOf_eqb_eq
-      func_eqb_eq
-      VDecl_eqb_eq
-      TVDecl_eqb_eq
-      DTDecl_eqb_eq
-    : Hints_soundness.
+  Create HintDb Hints_soundness.
+  Hint Resolve
+    string_eqb_eq
+    Recursivity_eqb_eq
+    Strictness_eqb_eq
+    Kind_eqb_eq
+    Ty_eqb_eq
+    some_valueOf_eqb_eq
+    func_eqb_eq
+    VDecl_eqb_eq
+    TVDecl_eqb_eq
+    DTDecl_eqb_eq
+  : Hints_soundness.
 
 
 
-    Lemma is_cong_Binding_Compat_Binding : ∀ b b',
-        (∀ t t', dec_R t t' = true -> R t t') ->
-        is_cong_binding b b' = true -> Compat_Binding b b'.
-    Proof with eauto with reflection.
-      intros b b' H_term_sound H_dec.
-      destruct b, b'.
-      all: simpl in H_dec; try discriminate H_dec.
-      all: split_hypos.
-      - assert (s = s0)...
-        assert (v = v0)...
-        subst.
-        apply C_TermBind...
-      - assert (t = t1)...
-        assert (t0 = t2)...
-        subst.
-        apply C_TypeBind.
-      - assert (d = d0)...
-        subst.
-        apply C_DatatypeBind.
-    Qed.
-
-    Lemma is_cong_Bindings_Compat_Bindings : ∀ bs bs',
-        (∀ t t', dec_R t t' = true -> R t t') ->
-        forall2b is_cong_binding bs bs' = true -> Compat_Bindings bs bs'.
-    Proof with eauto.
-      intros bs.
-      induction bs.
-      all: intros bs' H_term_sound H_dec.
-      all: destruct bs'.
-      all: simpl in H_dec.
-      all: try discriminate H_dec.
-      - apply Compat_Bindings_Nil.
-      - split_hypos.
-        apply Compat_Bindings_Cons.
-        + apply is_cong_Binding_Compat_Binding...
-        + eauto.
-    Qed.
-
-    Lemma is_cong_Compat t t' :
+  Lemma dec_compat_Binding_Compat_Binding : ∀ b b',
       (∀ t t', dec_R t t' = true -> R t t') ->
-      is_cong t t' = true -> Compat t t'.
-    Proof with eauto with reflection.
-      generalize t'.
-      clear t'.
-      intros t'.
-      induction t.
-      all: intros H_sound_R H_dec.
-      all: destruct t'.
-      all: simpl in H_dec.
-      all: try discriminate H_dec.
-      all: split_hypos.
-      - apply H_sound_R in H0.
-        apply Recursivity_eqb_eq in H.
-        subst.
-        eapply C_Let...
-        apply is_cong_Bindings_Compat_Bindings...
-      - apply String.eqb_eq in H_dec.
-        subst.
-        constructor.
-      - assert (b = s)...
-        assert (k = k0)...
-        subst.
-        eapply C_TyAbs...
-      - assert (b = s)...
-        assert (t = t1)...
-        subst.
-        apply C_LamAbs...
-      - apply C_Apply...
-      - assert (s = s0)...
-        subst.
-        apply C_Constant.
-      - assert (d = d0)... subst.
-        apply C_Builtin.
-      - assert (t0 = t1)... subst.
-        apply C_TyInst...
-      - assert (t = t0)... subst.
-        apply C_Error.
-      - assert (t = t2)...
-        assert (t0 = t3)...
-        subst.
-        apply C_IWrap...
-      - apply C_Unwrap...
-    Qed.
+      dec_compat_binding b b' = true -> Compat_Binding b b'.
+  Proof with eauto with reflection.
+    intros b b' H_term_sound H_dec.
+    destruct b, b'.
+    all: simpl in H_dec; try discriminate H_dec.
+    all: split_hypos.
+    - assert (s = s0)...
+      assert (v = v0)...
+      subst.
+      apply C_TermBind...
+    - assert (t = t1)...
+      assert (t0 = t2)...
+      subst.
+      apply C_TypeBind.
+    - assert (d = d0)...
+      subst.
+      apply C_DatatypeBind.
+  Qed.
+
+  Lemma dec_compat_Bindings_Compat_Bindings : ∀ bs bs',
+      (∀ t t', dec_R t t' = true -> R t t') ->
+      forall2b dec_compat_binding bs bs' = true -> Compat_Bindings bs bs'.
+  Proof with eauto.
+    intros bs.
+    induction bs.
+    all: intros bs' H_term_sound H_dec.
+    all: destruct bs'.
+    all: simpl in H_dec.
+    all: try discriminate H_dec.
+    - apply Compat_Bindings_Nil.
+    - split_hypos.
+      apply Compat_Bindings_Cons.
+      + apply dec_compat_Binding_Compat_Binding...
+      + eauto.
+  Qed.
+
+  Lemma sound_dec_compat t t' :
+    (∀ t t', dec_R t t' = true -> R t t') ->
+    dec_compat t t' = true -> Compat t t'.
+  Proof with eauto with reflection.
+    generalize t'.
+    clear t'.
+    intros t'.
+    induction t.
+    all: intros H_sound_R H_dec.
+    all: destruct t'.
+    all: simpl in H_dec.
+    all: try discriminate H_dec.
+    all: split_hypos.
+    - apply H_sound_R in H0.
+      apply Recursivity_eqb_eq in H.
+      subst.
+      eapply C_Let...
+      apply dec_compat_Bindings_Compat_Bindings...
+    - apply String.eqb_eq in H_dec.
+      subst.
+      constructor.
+    - assert (b = s)...
+      assert (k = k0)...
+      subst.
+      eapply C_TyAbs...
+    - assert (b = s)...
+      assert (t = t1)...
+      subst.
+      apply C_LamAbs...
+    - apply C_Apply...
+    - assert (s = s0)...
+      subst.
+      apply C_Constant.
+    - assert (d = d0)... subst.
+      apply C_Builtin.
+    - assert (t0 = t1)... subst.
+      apply C_TyInst...
+    - assert (t = t0)... subst.
+      apply C_Error.
+    - assert (t = t2)...
+      assert (t0 = t3)...
+      subst.
+      apply C_IWrap...
+    - apply C_Unwrap...
+  Qed.
 
 End Compatibility.
