src/Language/PlutusIR/Transform/DeadCode/Decide.v
@@ -28,12 +28,12 @@ Section Bindings.
     | b, b' => Binding_eqb b b'
     end.
 
-  Definition safely_removed b bs' :=
+  Definition dec_removed b bs' :=
     if negb (existsb (String.eqb (name_Binding b)) bs')
-      then is_pure_binding [] b
+      then dec_pure_binding [] b
       else true.
 
-  Definition binding_was_there b' bs : bool :=
+  Definition dec_was_present b' bs : bool :=
     match find (λ b, String.eqb (name_Binding b) (name_Binding b')) bs with
       | Datatypes.Some b => dec_elim_Binding b b'
       | None => false
@@ -48,32 +48,12 @@ Section Bindings.
     | b :: bs => if String.eqb (name_Binding b) (name_Binding b') then dec_elim_Binding b b' else find bs
     end.
 
-  (* This does not work in the termination checker, it doesn't see that b returned by find 
-     is a structural subterm.
-     It would have to fuse the result of find (an option string) with the resulting, which is
-     what I did in the above definition*)
-  Definition find_Binding' b' bs :=
-    match find (λ b, String.eqb (name_Binding b) (name_Binding b')) bs with
-      | Datatypes.Some b => dec_elim_Binding b b'
-      | None => false
-    end.
-
-
   Definition dec_elim_Bindings (bs bs' : list Binding) : bool :=
     let bsn := map name_Binding bs in
     let bs'n := map name_Binding bs' in
-    forallb (fun b => safely_removed b bs'n) bs &&
+    forallb (fun b => dec_removed b bs'n) bs &&
     forallb (fun b' => find_Binding b' bs) bs'.
 
-  (* this did not pass termination checking *)
-  (*
-    forallb (fun b' =>
-    match find (λ b, String.eqb (name_Binding b) (name_Binding b')) bs with
-      | Datatypes.Some b => dec_elim_Binding b b'
-      | None => false
-    end
-    ) bs'
-   *)
 End Bindings.
 
 Fixpoint dec_elim_Term (x y : Term) {struct x} : bool := match x, y with
@@ -83,10 +63,10 @@ Fixpoint dec_elim_Term (x y : Term) {struct x} : bool := match x, y with
       then (* same let block, but bindings were removed *)
         Recursivity_eqb r r' && dec_elim_Term t t'
       else (* t' is another let block, the whole block in the pre-term was removed *)
-        forallb (is_pure_binding []) bs && dec_elim_Term t y (* Check whether the whole let was removed *)
+        forallb (dec_pure_binding []) bs && dec_elim_Term t y (* Check whether the whole let was removed *)
   | Let _ bs t   , _ => 
-     forallb (is_pure_binding []) bs && dec_elim_Term t y (* Check whether the whole let was removed *)
-  | _ , _ => is_cong dec_elim_Term x y
+     forallb (dec_pure_binding []) bs && dec_elim_Term t y (* Check whether the whole let was removed *)
+  | _ , _ => dec_compat dec_elim_Term x y
 
   end
 .
